confluence.v
@@ -1,0 +1,46 @@
+(** Confluence of beta-reduction in combinatory algebra.
+
+    TODO declare [red] to be reflexive and transitive,
+    as described in https://coq.inria.fr/refman/Reference-Manual029.html
+*)
+
+Inductive term :=
+  | S : term
+  | K : term
+  | AP : term -> term -> term.
+Hint Constructors term.
+
+Notation "x * y" := (AP x y) (at level 40, left associativity).
+
+Inductive step : term -> term -> Prop :=
+  | step_s: forall x y z, step (S * x * y * z) (x * z * (y * z))
+  | step_k: forall x y, step (K * x * y) x
+  | step_ap_1: forall x x0 y, step x x0 -> step (x * y) (x0 * y)
+  | step_ap_2: forall x y y0, step y y0 -> step (x * y) (x * y0).
+Hint Constructors step.
+
+Inductive red : term -> term -> Prop :=
+  | red_refl: forall x, red x x
+  | red_trans: forall x y z, red x y -> step y z -> red x z.
+Hint Constructors red.
+
+Lemma confluence_step_step:
+  forall x y y0,
+  step x y -> step x y0 -> exists z, red y z /\ red y0 z.
+Proof.
+  intros.
+  inversion H; inversion H0.
+  exists (x0 * z * (y1 * z)).
+  split; reflexivity.
+  auto.
+  apply step_s .
+
+
+Theorem confluence:
+  forall x y y0,
+  red x y -> red x y0 -> exists z, red y z /\ red y0 z.
+Proof.
+  intros.
+  (* TODO *)
+Qed.
+
